removed \McR from SnNor

LeanStlc/StrongNorm3.lean
@@ -6,7 +6,7 @@ import LeanStlc.Preservation
 
 open LeanSubst
 
-namespace StrongNormalizaton3
+namespace StrongNormalization3
 
 def Set A := A -> Prop
 
@@ -18,7 +18,7 @@ def ℛ (S : Set Term) : Set Term
 mutual
   @[grind]
   inductive SnNor : Set Term -> Term -> Prop
-  | lam : ℛ S (:λ[A] t) -> SnNor S t -> SnNor S (:λ[A] t)
+  | lam : S1 (:λ[A] t) -> SnNor S2 t -> SnNor S1 (:λ[A] t) -- I got rid of the ℛ
   | zero : SnNor S .zero
   | succ : SnNor S t -> SnNor S t.succ
   | neu : SnNeu S t -> SnNor S t
@@ -27,16 +27,16 @@ mutual
   @[grind]
   inductive SnNeu : Set Term -> Term -> Prop
   | var : SnNeu S #x
-  | app : SnNeu S s -> SnNor S t -> SnNeu S (s :@ t)
-  | nrec : SnNor S z -> SnNor S s -> SnNeu S t -> SnNeu S (.nrec A z s t)
+  | app : SnNeu S1 s -> SnNor S2 t -> SnNeu S3 (s :@ t)
+  | nrec : SnNor S1 z -> SnNor S2 s -> SnNeu S3 t -> SnNeu S4 (.nrec A z s t)
 
   @[grind]
   inductive SnRed : Set Term -> Term -> Term -> Prop
-  | beta : SnNor S t -> SnRed S ((:λ[A] b) :@ t) b[su t::+0]
-  | zero : SnNor S s -> SnRed S (.nrec A z s .zero) z
+  | beta : SnNor S1 t -> SnRed S2 ((:λ[A] b) :@ t) b[su t::+0]
+  | zero S1 : SnNor S1 s -> SnRed S2 (.nrec A z s .zero) z
   | succ : SnRed S (.nrec A z s t.succ) (s :@ (.nrec A z s t))
-  | step_app : SnRed S s s' -> SnRed S (s :@ t) (s' :@ t)
-  | step_nrec : SnRed S n n' -> SnRed S (.nrec A z s n) (.nrec A z s n')
+  | step_app : SnRed S1 s s' -> SnRed S2 (s :@ t) (s' :@ t)
+  | step_nrec : SnRed S1 n n' -> SnRed S2 (.nrec A z s n) (.nrec A z s n')
 end
 
 @[simp]
@@ -50,43 +50,275 @@ instance : Model $ Set Term where
   P := Set.empty
   N := Set.empty
 
-def ℰ A := SnNor ⟦ A ⟧
+@[simp]
+def 𝒱 (Γ : List Ty) : Ty -> Set Term
+| (A -t> B) =>
+  λ x => match x with
+  | :λ[_] t => ∀ a, Γ ⊢ a : A -> SnNor (𝒱 Γ A) a -> (A :: Γ) ⊢ t : B -> SnNor (𝒱 Γ B) t[su a::+0]
+  | _ => False
+| _ => Set.empty
 
-def 𝒞 (Γ : List Ty) (σ : Subst Term) : Prop :=
-  ∀ {i T}, Γ[i]? = .some T -> ℰ T (σ i)
+def ℰ Γ A := λ t => Γ ⊢ t : A ∧ SnNor (𝒱 Γ A) t
+
+def 𝒞 (Γ : List Ty) (Δ : List Ty) (σ : Subst Term) : Prop :=
+  ∀ {i T}, Γ[i]? = .some T -> ℰ Δ T (σ i)
 
 @[simp]
 def SemanticTyping (Γ : List Ty) (t : Term) (A : Ty) :=
-  ∀ σ, 𝒞 Γ σ -> ℰ A t[σ]
+  ∀ σ Δ, 𝒞 Γ Δ σ -> ℰ Δ A t[σ]
 
 local notation:170 Γ:170 " ⊨ " t:170 " : " A:170 => SemanticTyping Γ t A
 
-theorem lam : ℛ ⟦A -t> B⟧ (:λ[C] b) <-> ∀ (r:Ren) a, ℰ A a -> ℰ B b[su a::r.to] := by
-  sorry
+theorem SnRed.preservation : Γ ⊢ t : A -> SnRed S t t' -> Γ ⊢ t' : A
+| Typing.app (Typing.lam j1) j2, SnRed.beta h1 => Typing.beta j1 j2
+| Typing.app j1 j2, .step_app h1 => Typing.app (SnRed.preservation j1 h1) j2
+| Typing.nrec j1 j2 (Typing.succ j3), .succ => Typing.app j2 (Typing.nrec j1 j2 j3)
+| Typing.nrec j1 _ _, .zero S1 h1 => j1
+| Typing.nrec j1 j2 j3, .step_nrec h1 => Typing.nrec j1 j2 (SnRed.preservation j3 h1)
+
+-- theorem lam1 : ℛ ⟦A -t> B⟧ (:λ[C] b) -> Γ ⊢ (:λ[C] b) : (A -t> B) -> ∀ (r:Ren) a, Γ -⟨r⟩> Δ -> ℰ Δ A a -> ℰ Δ B b[su a::r.to]
+-- | h1, h3, r, a, h2, h4 =>
+--   by
+--     simp only [ℛ] at h1; replace h1 := h1 r; simp at h1;
+--     apply And.intro _
+--     apply h1; exact h4.2
+--     cases h3
+--     case _ h3 =>
+--       replace h2 : Γ -[r.to]> Δ := h2.to
+--       replace h2 : (A :: Γ) -[su a :: r.to]> Δ := TypingSubst.su h4.1 h2
+--       apply Typing.subst h2 h3
+
+-- theorem lam2 : (∀ (r:Ren) a, Γ -⟨r⟩> Δ -> ℰ Δ A a -> ℰ Δ B b[su a::r.to]) -> (ℛ ⟦A -t> B⟧ (:λ[C] b) ∧ Γ ⊢ (:λ[C] b) : (A -t> B)) := by
+--   intro h
+--   apply And.intro
+--   intro r
+--   simp
+
+theorem SnNor.appl : ∀ {A B a}, (S = 𝒱 Γ (A -t> B)) -> Γ ⊢ a : (A -t> B) ->  SnNor S a -> ℰ Γ A b -> ℰ Γ B (a :@ b)
+| A, B, :λ[_] t, eq, .lam j1, SnNor.lam h1 h2, ⟨j2, j3⟩ =>
+  let lem2 : (λ x => x) = @id Nat:= by unfold id; rfl
+  let lem : SnNor (𝒱 Γ B) t[su b :: +0] := by
+    --simp only [ℛ] at h1
+    subst eq
+    simp only [𝒱] at h1
+    simp at h1
+    apply h1; apply j2; apply j3; apply j1
+  ⟨Typing.app (.lam j1) j2, SnNor.red (SnRed.beta j3) lem⟩
+| A, B, a, eq, j1, .neu h1, ⟨j2, j3⟩ => ⟨Typing.app j1 j2, SnNor.neu (SnNeu.app h1 j3)⟩
+| A, B, f, eq, j1, .red h1 h2, ⟨j2, j3⟩ => ⟨Typing.app j1 j2, SnNor.red (SnRed.step_app h1) (SnNor.appl eq (SnRed.preservation j1 h1) h2 ⟨j2, j3⟩ ).2⟩
 
 theorem ℰ.nrec :
-  ℰ A z ->
-  ℰ (A -t> A) s ->
-  ℰ Ty.nat n ->
-  ℰ A (.nrec A z s n)
-:= by
-  sorry
+  ℰ Γ A z ->
+  ℰ Γ (A -t> A) s ->
+  S = ⟦ Ty.nat ⟧ ->
+  Γ ⊢ n : Ty.nat ->
+  SnNor S n ->
+  ℰ Γ A (.nrec A z s n)
+| ⟨j1, j2⟩, ⟨j3, j4⟩, _, j5, .zero => ⟨Typing.nrec j1 j3 j5, SnNor.red (SnRed.zero _ j4) j2⟩
+| ⟨j1, j2⟩, ⟨j3, j4⟩, eq, Typing.succ j5, .succ h1 => ⟨Typing.nrec j1 j3 (Typing.succ j5) , SnNor.red (SnRed.succ) (SnNor.appl rfl j3 j4 (ℰ.nrec ⟨j1, j2⟩ ⟨j3, j4⟩ eq j5 h1)).2⟩
+| ⟨j1, j2⟩, ⟨j3, j4⟩, _, j5, .neu h1 => ⟨Typing.nrec j1 j3 j5, SnNor.neu (SnNeu.nrec j2 j4 h1)⟩
+| ⟨j1, j2⟩, ⟨j3, j4⟩, eq, j5, .red h1 h2 => ⟨Typing.nrec j1 j3 j5, SnNor.red (SnRed.step_nrec h1) (ℰ.nrec ⟨j1, j2⟩ ⟨j3,j4⟩ eq (SnRed.preservation j5 h1) h2).2⟩
+
+theorem context_renaming : 𝒞 Γ Δ σ -> Γ ⊢ t : A -> Δ ⊢ t[σ] : A
+| h1, h2 =>
+  let lem : ∀ {i : Nat} {T : Ty}, Γ[i]? = some T → Δ ⊢ ↑(σ i) : T := by
+    intro i T j1
+    have h1 := h1 j1
+    simp only [ℰ] at h1
+    rcases h1 with ⟨e1, e2⟩
+    exact e1
+  Typing.subst lem h2
+
+theorem context_to_typingsubst : 𝒞 Γ Δ σ -> (∀ {x T}, Γ[x]? = some T -> Δ ⊢ σ x : T)
+| h1, _, _, h2 => (h1 h2).1
+
+mutual
+  theorem SnNor.lift {σ : Subst Term} :
+    SnNor (𝒱 Δ T) (σ n) ->
+    SnNor (𝒱 (A :: Δ) T) (σ.lift (n + 1))
+  := by
+    intro h1
+    generalize zdef : (σ n) = z
+    rw [zdef] at h1
+    cases z
+    case _ =>
+      cases n
+      case _ =>
+        unfold Subst.lift
+        simp
+        rw [zdef]
+        simp
+        apply SnNor.neu
+        apply SnNeu.var
+      case _ =>
+        unfold Subst.lift
+        simp
+        rw [zdef]
+        simp
+        apply SnNor.neu
+        apply SnNeu.var
+    case _ t =>
+      cases h1
+      case _ S2 t A' h1 h2 =>
+        unfold Subst.lift
+        simp
+        rw [zdef]
+        simp
+        sorry
+      case _ =>
+        sorry
+      case _ =>
+        sorry
+      case _ =>
+        sorry
+      case _ =>
+        sorry
+
+  theorem SnNeu.lift {σ : Subst Term} :
+    SnNeu (𝒱 Δ T) (σ n) ->
+    SnNeu (𝒱 (A :: Δ) T) (σ.lift (n + 1))
+  := by
+    sorry
+end
+
+theorem context_lift : 𝒞 Γ Δ σ -> 𝒞 (A :: Γ) (A :: Δ) σ.lift
+| h1, 0, _, h4 => ⟨TypingSubst.lift (Γ := Γ) (Δ := Δ) (σ := σ) A (λ x => (h1 x).1) h4, (SnNor.neu (SnNeu.var))⟩
+| h1, _ + 1, _, h4 => ⟨TypingSubst.lift (Γ := Γ) (Δ := Δ) (σ := σ) A (λ x => (h1 x).1) h4, SnNor.lift (h1 h4).2⟩
+
+-- mutual
+--   def SnNor.rename (r : Ren) : SnNor S t -> SnNor S t[r]
+--   | @SnNor.lam S1 S2 t A f th =>
+--     let lem : SnNor S2 t[r.to.lift] := by
+--       rw [<-Ren.to_lift]
+--       exact .rename r.lift th
+--     let lem2 : S1 (:λ[A] t[r.to.lift]) := by
+--       --rw [<-Ren.to_lift]
+--       simp only [ℛ] at *
+--       intro r'
+--       simp at *
+--       apply f
+--     SnNor.lam lem2 lem
+--   | .zero => .zero
+--   | .succ t => .succ (t.rename r)
+--   | .neu t => .neu (t.rename r)
+--   | .red h t' => .red (h.rename r) (t'.rename r)
+
+--   def SnNeu.rename (r : Ren) : SnNeu S t -> SnNeu S t[r]
+--   | .var => .var
+--   | .app s t => .app (s.rename r) (t.rename r)
+--   | .nrec t z s => .nrec (t.rename r) (z.rename r) (s.rename r)
+
+--   def SnRed.rename (r : Ren) : SnRed S t t' -> SnRed S t[r] t'[r]
+--   | @SnRed.beta S1 t S2 A b th => by {
+--     have lem := @SnRed.beta S1 (t[r]) S2 A (b[.re 0 :: r ∘ +1]) (.rename r th)
+--     simp at lem; simp; exact lem
+--   }
+--   | .zero S1 h => .zero S1 (h.rename r)
+--   | .succ => .succ
+--   | .step_app h => .step_app (h.rename r)
+--   | .step_nrec h => .step_nrec (h.rename r)
+-- end
+
+@[simp]
+theorem test : Term.smap σ t = t[σ] := by
+  induction t
+  case _ =>
+    simp
+  case _ ih1 ih2 =>
+    simp
+    apply And.intro
+    apply ih1
+    apply ih2
+  case _ A t ih =>
+    simp
+    unfold Term.smap
+    sorry
+  case _ =>
+    simp
+  case _ ih =>
+    simp
+    apply ih
+  case _ ih1 ih2 ih3 =>
+    simp
+    apply And.intro; apply ih1; apply And.intro; apply ih2; apply ih3
 
 theorem fundamental : Γ ⊢ t : A -> Γ ⊨ t : A
-| .var xj, σ, h =>  h xj
-| .app fj aj, σ, h =>
-  sorry
-| .lam tj, σ, h =>
+| .var xj, σ, Δ, h =>  h xj
+| .app fj aj, σ, Δ, h =>
+  let fj' := (fundamental fj) σ Δ
+  let aj' := (fundamental aj) σ Δ
+  by simp; apply SnNor.appl rfl (by apply context_renaming h fj) (fj' h).2 (aj' h)
+| .lam (A := A') (B := B) (t := t) tj, σ, Δ, h =>
   let nj' := fundamental tj
-  .lam sorry sorry
-| .zero, σ, h => .zero
-| .succ nj, σ, h =>
-  let nj' := fundamental nj σ h
-  .succ nj'
-| .nrec zj sj nj, σ, h =>
-  let zj' := fundamental zj σ h
-  let sj' := fundamental sj σ h
-  let nj' := fundamental nj σ h
-  ℰ.nrec zj' sj' nj'
+  let lem : (𝒱 Δ (A' -t> B)) (:λ[A'] t[σ.lift]) := by
+    intro a j1 j2 j3
+    simp at *
+    let lem2 : 𝒞 (A' :: Γ) Δ (su a :: σ) := by
+      unfold 𝒞 at *
+      intro i T w
+      unfold ℰ at *
+      apply And.intro
+      case _ =>
+        cases i
+        case _ =>
+          simp
+          simp at w
+          subst w
+          apply j1
+        case _ n =>
+          let lem3 : σ n = (su a :: σ) (n + 1) := by simp
+          let lem4 : Γ[n]? = (A' :: Γ)[n + 1]? := by simp
+          replace h :=@ h n T
+          rw [lem4] at h
+          rw [lem3] at h
+          replace h := h w
+          apply h.1
+      case _ =>
+        cases i
+        case _ =>
+          simp
+          simp at w
+          subst w
+          apply j2
+        case _ n =>
+          replace h := @h n T
+          let lem3 : σ n = (su a :: σ) (n + 1) := by simp
+          let lem4 : Γ[n]? = (A' :: Γ)[n + 1]? := by simp
+          rw [lem4] at h
+          rw [lem3] at h
+          replace h := h w
+          apply h.2
+    replace nj' := nj' (su a :: σ) Δ lem2
+    apply nj'.2
+  ⟨context_renaming h (Typing.lam tj),
+   SnNor.lam (S2 := (𝒱 (A'::Δ) B)) lem (nj' _ (A'::Δ) (context_lift h)).2⟩
+  -- let jj := TypingSubst.lift (Γ := Γ) (Δ := Δ) (σ := σ) (A := A')
+  -- have lem : ∀ {x T}, Γ[x]? = some T -> Δ ⊢ σ x :T := by
+  --   intro x T h2
+  --   simp only [𝒞] at h
+  --   replace h := @h x T h2
+  --   simp only [ℰ] at h
+  --   rcases h with ⟨e1,e2⟩
+  --   apply e1
+  -- have lem2 : 𝒞 (A' :: Γ) (A' :: Δ) σ.lift := by
+  --   apply context_lift
+  --   apply h
+  -- have lem3 : ∀ a (r : Ren), 𝒞 (A' :: Γ) (Δ) (su a :: σ ∘ r.to) := by
+  --   intro a r
+  --   apply context_shift
+  --   apply h
+  -- ⟨Typing.lam (context_renaming
+  -- (by intro i T h2; simp only [ℰ]; unfold TypingSubst at *; simp only [𝒞, ℰ] at lem2; replace lem2 := @lem2 i T h2; exact lem2) tj), SnNor.lam (S2 := ⟦ B ⟧)
+  -- (by sorry)
+  -- (by simp at nj'; simp only [ℰ] at nj'; unfold TypingSubst at *; replace nj' := nj' σ.lift (A'::Δ) lem2; rcases nj' with ⟨e1,e2⟩; exact e2)⟩
+| .zero, σ, Δ, h => ⟨Typing.zero, SnNor.zero⟩
+| .succ nj, σ, Δ, h =>
+  let nj' := fundamental nj σ Δ h
+  ⟨Typing.succ nj'.1, SnNor.succ nj'.2⟩
+| .nrec zj sj nj, σ, Δ, h =>
+  let zj' := fundamental zj σ Δ h
+  let sj' := fundamental sj σ Δ h
+  let nj' := fundamental nj σ Δ h
+  ℰ.nrec zj' sj' rfl nj'.1 nj'.2
 
-namespace StrongNormalizaton3
+namespace StrongNormalization3
